code/experimental/rsapss/Hacl.Impl.Bignum.Division.fst
@@ -10,25 +10,74 @@ open LowStar.Buffer
 open Lib.IntTypes
 open Lib.Buffer
 
-open Hacl.Impl.Bignum.Core
-open Hacl.Impl.Bignum.Convert
-open Hacl.Impl.Bignum.Shift
-open Hacl.Impl.Bignum.Comparison
-open Hacl.Impl.Bignum.Multiplication
 open Hacl.Impl.Bignum.Addition
+open Hacl.Impl.Bignum.Core
+open Hacl.Impl.Bignum.Misc
 open Hacl.Spec.Bignum
 
 
+// Naive binary non constant-time division. To be improved later.
+// It's inspired by the boringssl, should I add the copyright notice?
+
+
+// Sets a to (a mod m), where a < 2 * m. Returns (-1) if reduction was
+// performed (a >= m), otherwise 0.
+// a may have an additional word specified by carry.
+val bn_reduce_once_in_place:
+     #nLen:bn_len
+  -> a:lbignum nLen
+  -> carry:uint64
+  -> m:lbignum nLen
+  -> tmp:lbignum nLen
+  -> Stack uint64
+    (requires fun h ->
+     live h a /\ live h m /\ live h tmp /\
+     all_disjoint [loc a; loc m; loc tmp])
+    (ensures fun h0 _ h1 -> modifies2 a tmp h0 h1)
+let bn_reduce_once_in_place #nLen a carry m tmp =
+  let carry2 = bn_sub a m tmp in
+  let carry' = carry -. carry2 in
+  if eq_u64 carry' (uint 0) then copy a tmp;
+  carry'
+
+#reset-options "--z3rlimit 100 --max_fuel 0 --max_ifuel 0"
+
 val bn_divide:
      #aLen:bn_len
-  -> #bLen:bn_len
   -> a:lbignum aLen
-  -> b:lbignum bLen
-  -> res:lbignum aLen
+  -> b:lbignum aLen
+  -> q:lbignum aLen
+  -> r:lbignum aLen
   -> Stack unit
     (requires fun h ->
-     live h a /\ live h b /\ all_disjoint [loc a; loc b; loc res] /\
+     live h a /\ live h b /\ live h q /\ live h r /\
+     all_disjoint [loc a; loc b; loc q; loc r] /\
      as_snat h b <> 0)
-    (ensures fun h0 _ h1 -> modifies1 res h0 h1 /\
-      as_snat h1 res = as_snat h0 a / as_snat h0 b)
-let bn_divide #aLen #bLen a b res = admit()
+    (ensures fun h0 _ h1 -> modifies2 q r h0 h1 /\
+      as_snat h1 q = as_snat h0 a / as_snat h0 b /\
+      as_snat h1 r = as_snat h0 a % as_snat h0 b)
+let bn_divide #aLen a b q r =
+  push_frame ();
+
+  let tmp = create aLen (u64 0) in
+  bn_assign_uint64 q (uint 0);
+  bn_assign_uint64 r (uint 0);
+
+  let h0 = FStar.HyperStack.ST.get () in
+  let inv1 h i = modifies3 q r tmp h0 h in
+  let inv2 h i = modifies3 q r tmp h0 h in
+
+  Lib.Loops.for_rev aLen 0ul inv1 (fun i ->
+    Lib.Loops.for_rev 64ul 0ul inv2 (fun bit ->
+      let carry = bn_add r r r in
+      r.(0ul) <- r.(0ul) |. ((a.(i) >>. bit) &. (u64 1));
+      let subtracted = bn_reduce_once_in_place r carry b tmp in
+      q.(i) <- q.(i) |. (((~. subtracted) &. (u64 1)) <<. bit)
+  ));
+
+  let h = FStar.HyperStack.ST.get () in
+
+  assume (as_snat h q = as_snat h0 a / as_snat h0 b /\
+          as_snat h r = as_snat h0 a % as_snat h0 b);
+
+  pop_frame ()
